operations_refine.v
@@ -24,35 +24,36 @@ Lemma addr_alive_refine' Γ α f m1 m2 a1 a2 σp :
   index_alive' m1 (addr_index a1) → a1 ⊑{Γ,α,f@'{m1}↦'{m2}} a2 : σp →
   index_alive' m2 (addr_index a2).
 Proof. eauto using addr_alive_refine. Qed.
-Lemma addr_eq_ok_refine Γ α f m1 m2 a1 a2 a3 a4 σp :
+Lemma addr_compare_ok_refine Γ α f m1 m2 c a1 a2 a3 a4 σp :
   a1 ⊑{Γ,α,f@'{m1}↦'{m2}} a2 : σp → a3 ⊑{Γ,α,f@'{m1}↦'{m2}} a4 : σp →
-  addr_eq_ok Γ m1 a1 a3 → addr_eq_ok Γ m2 a2 a4.
+  addr_compare_ok Γ m1 c a1 a3 → addr_compare_ok Γ m2 c a2 a4.
 Proof.
-  intros Ha1 Ha2 (?&?&?); split_ands'; eauto using addr_alive_refine'; intros.
-  destruct (decide (addr_index a1 = addr_index a3));
+  intros Ha1 Ha2 (?&?&?); split_ands'; eauto using addr_alive_refine'.
+  intros. destruct (decide (addr_index a1 = addr_index a3));
     [destruct Ha1, Ha2; naive_solver|intuition eauto using addr_strict_refine].
 Qed.
-Lemma addr_eq_refine Γ α f m1 m2 a1 a2 a3 a4 σp :
-  ✓ Γ → addr_eq_ok Γ m1 a1 a3 →
+Lemma addr_compare_refine Γ α f m1 m2 c a1 a2 a3 a4 σp :
+  ✓ Γ → addr_compare_ok Γ m1 c a1 a3 →
   a1 ⊑{Γ,α,f@'{m1}↦'{m2}} a2 : σp → a3 ⊑{Γ,α,f@'{m1}↦'{m2}} a4 : σp →
-  addr_eq Γ a1 a3 = addr_eq Γ a2 a4.
+  addr_compare Γ c a1 a3 = addr_compare Γ c a2 a4.
 Proof.
-  intros ? (_&_&Hstrict) Ha1 Ha2; unfold addr_eq.
+  intros ? (_&_&Hstrict) Ha1 Ha2; unfold addr_compare; apply bool_decide_iff.
   assert ('{m1} ⊑{Γ,α,f} '{m2}) as HΔ by eauto using addr_refine_memenv_refine.
   destruct (addr_object_offset_refine Γ α f
     ('{m1}) ('{m2}) a1 a2 σp) as (r1&?&?&->); auto.
   destruct (addr_object_offset_refine Γ α f
     ('{m1}) ('{m2}) a3 a4 σp) as (r3&?&?&->); auto.
-  destruct (decide (addr_index a1 = addr_index a3)); [|destruct Hstrict; auto].
-  { rewrite decide_True by congruence. replace r1 with r3 by congruence.
-    apply bool_decide_iff; omega. }
-  destruct (decide (addr_index a2 = addr_index a4)) as [Ha|]; [|done].
-  apply eq_sym, bool_decide_false. destruct (meminj_injective_alt f
-    (addr_index a1) (addr_index a3) (addr_index a2) r1 r3) as [|[_ ?]];
+  destruct (decide (addr_index a1 = addr_index a3)).
+  { replace r1 with r3 by congruence. clear Hstrict.
+    destruct c; simplify_equality'; intuition auto with congruence lia. }
+  split; [by intros []|intros [Ha ?]].
+  destruct Hstrict as (->&?&?); auto; csimpl in *.
+  destruct (meminj_injective_alt f (addr_index a1) (addr_index a3)
+    (addr_index a2) r1 r3) as [|[_ ?]];
     eauto using memenv_refine_injective with congruence.
   assert (addr_object_offset Γ a1 < bit_size_of Γ (addr_type_object a1) ∧
     addr_object_offset Γ a3 < bit_size_of Γ (addr_type_object a3)) as []
-    by eauto using addr_object_offset_strict.
+    by intuition eauto using addr_object_offset_strict.
   assert (addr_type_object a2 = addr_type_object a4).
   { eapply typed_unique; eauto using addr_typed_index.
     rewrite Ha; eauto using addr_typed_index. }
@@ -136,15 +137,14 @@ Lemma ptr_compare_ok_refine Γ α f m1 m2 c p1 p2 p3 p4 σp :
   ptr_compare_ok Γ m1 c p1 p3 → ptr_compare_ok Γ m2 c p2 p4.
 Proof.
   destruct 1, 1, c; simpl; eauto using addr_minus_ok_refine,
-    addr_alive_refine, addr_eq_ok_refine.
+    addr_alive_refine, addr_compare_ok_refine.
 Qed.
 Lemma ptr_compare_refine Γ α f m1 m2 c p1 p2 p3 p4 σp :
   ✓ Γ → ptr_compare_ok Γ m1 c p1 p3 →
   p1 ⊑{Γ,α,f@'{m1}↦'{m2}} p2 : σp → p3 ⊑{Γ,α,f@'{m1}↦'{m2}} p4 : σp →
   ptr_compare Γ c p1 p3 = ptr_compare Γ c p2 p4.
 Proof.
-  destruct 3, 1, c; simpl; eauto 2 using addr_eq_refine;
-    by erewrite addr_minus_refine by eauto.
+  destruct 3, 1; simpl; repeat case_match; eauto 2 using addr_compare_refine.
 Qed.
 Lemma ptr_plus_ok_refine Γ α f m1 m2 p1 p2 σp j :
   p1 ⊑{Γ,α,f@'{m1}↦'{m2}} p2 : σp →
